tweaks, still stuck on Neg Complete

coq/Inv.v
@@ -22,52 +22,61 @@ Open Scope list_scope.
 Axiom V : Type.
 Axiom V_eq_dec : forall (v1 v2: V), {v1 = v2} + {v1 <> v2}.
 Notation Ty := (Ensemble V).
-Definition IsEmpty (t:Ty) : Prop := ~ (Inhabited V t).
-Axiom IsEmpty_dec : forall (t: Ty), {IsEmpty t} + {~ IsEmpty t}.
+
+Notation emptyTy := (Empty_set V).
+Notation anyTy := (Full_set V).
+Notation tyOr := (Union V).
+Notation tyAnd := (Intersection V).
+Notation tyDiff := (Setminus V).
+Notation tyNot := (tyDiff anyTy).
+
+Notation IsEmpty t := (~ Inhabited V t).
+Notation IsInhabited t := (Inhabited V t).
+Axiom IsEmpty_dec : forall (t: Ty), {IsEmpty t} + {IsInhabited t}.
 Notation IsA v T := (In V T v).
 Axiom IsA_dec : forall (v:V) (t: Ty), {IsA v t} + {~ IsA v t}.
 Notation "T1 <: T2" := (Included V T1 T2) (at level 70).
 
-Definition emptyTy : Ty := Empty_set V.
-Definition anyTy : Ty := Full_set V.
-Definition tyOr : Ty -> Ty -> Ty := Union V.
-Definition tyAnd : Ty -> Ty -> Ty := Intersection V.
-Definition tyDiff : Ty -> Ty -> Ty := Setminus V.
-Definition tyNot : Ty -> Ty := tyDiff anyTy.
+Hint Unfold Included Setminus.
+Hint Constructors Union Intersection Inhabited.
 
-Hint Unfold emptyTy.
-Hint Unfold anyTy.
-Hint Unfold tyOr.
-Hint Unfold tyAnd.
-Hint Unfold tyDiff.
-Hint Unfold tyNot.
+
+Lemma no_empty_val : forall v,
+    ~ IsA v emptyTy.
+Proof.
+  intros v Hmt. inversion Hmt.
+Qed.
+
+
 
 (* A single function arrow *)
 Inductive arrow : Type :=
 | Arrow : Ty -> Ty -> arrow.
-
 Hint Constructors arrow.
 
 Definition a_meet (a1 a2 : arrow) : arrow :=
   match a1, a2 with
   | Arrow d1 r1, Arrow d2 r2 => Arrow (tyAnd d1 d2) (tyAnd r1 r2)
   end.
+Hint Unfold a_meet.
 
 Definition a_dom (a : arrow) : Ty :=
   match a with
   | Arrow t1 _ => t1
   end.
+Hint Unfold a_dom.
 
 Definition a_rng (a : arrow) : Ty :=
   match a with
   | Arrow _ t2 => t2
   end.
+Hint Unfold a_rng.
+
 
 Inductive res : Type :=
 | Err : res (* invalid argument/type error *)
 | Bot : res (* non-termination *)
 | Res : V -> res. (* a value result *)
-
 Hint Constructors res.
 
 Definition fn := (V -> res).
@@ -79,13 +88,193 @@ Inductive FnArrow : fn -> arrow -> Prop :=
         (f v = Bot
          \/ (exists v', IsA v' T2 /\ f v = Res v'))) ->
     FnArrow f (Arrow T1 T2).
-
 Hint Constructors FnArrow.
 
+
+Ltac destruct_IsA :=
+  match goal with
+  | [H : IsA _ _ |- _] => destruct H
+  end.
+
+Definition a_inv_pos (a:arrow) (out:Ty) : Ty :=
+  if (IsEmpty_dec (tyAnd (a_rng a) out))
+  then emptyTy
+  else (a_dom a).
+
+Definition a_inv_neg (a:arrow) (out:Ty) : Ty :=
+  if (IsEmpty_dec (tyAnd (a_rng a) out))
+  then (a_dom a)
+  else emptyTy.
+
+Hint Unfold a_inv_pos a_inv_neg.
+
+Definition ArrowInvPos 
+           (a:arrow)
+           (outT inT : Ty) : Prop :=
+forall (f:fn),
+  FnArrow f a ->
+  forall (v v':V),
+    IsA v (a_dom a) ->
+    f v = Res v' ->
+    IsA v' outT ->
+    IsA v inT.
+
+Definition ArrowInvNeg 
+           (a:arrow)
+           (outT inT : Ty) : Prop :=
+forall (f:fn),
+  FnArrow f a ->
+  forall (v v':V),
+    f v = Res v' ->
+    ~ (IsA v' outT /\ IsA v inT).
+
+Hint Unfold ArrowInvPos ArrowInvNeg.
+
+Ltac same_Res :=
+  match goal with
+  | [H1 : ?f ?v = Res ?x , H2 : ?f ?v = Res ?y |- _] =>
+    rewrite H1 in H2; inversion H2; subst; clear H2
+  end.
+
+Ltac inv_FnArrow :=
+  match goal with
+  | [H : FnArrow _ _ |- _] => inversion H; subst
+  end.
+
+
+(* Arrow Inversion Soundness *)
+Lemma a_inv_pos_sound : forall a outT inT,
+    a_inv_pos a outT = inT ->
+    ArrowInvPos a outT inT.
+Proof with crush.
+  unfold ArrowInvPos.
+  intros [T1 T2] outT inT Hinv f Hf v v' Hin Hfv Hout.
+  unfold a_inv_pos in *. simpl in *. 
+  destruct (IsEmpty_dec (tyAnd T2 outT)) as [Hmt | Hnmt]...
+  inv_FnArrow.
+  applyHinH...
+  same_Res.
+  assert (Inhabited V (tyAnd T2 outT)) as impossible...
+  exists x...
+Qed.
+
+Lemma a_inv_neg_sound : forall a outT inT,
+    a_inv_neg a outT = inT ->
+    ArrowInvNeg a outT inT.
+Proof with crush.
+  unfold ArrowInvNeg.
+  intros [T1 T2] outT inT Hinv f Hf v v' Hfv.
+  unfold a_inv_neg in *. simpl in *. 
+  destruct (IsEmpty_dec (tyAnd T2 outT)) as [Hmt | Hnmt]...
+  (* ~ IsInhabited (tyAnd T2 outT) *)
+  {
+    apply Hmt. exists v'. split; crush.
+    inv_FnArrow.
+    applyHinH...
+  }
+  (* IsInhabited (tyAnd T2 outT) *)
+  {
+    eapply no_empty_val; eauto.
+  }
+Qed.
+  
+  
+(* Arrow Inversion Completeness *)
+Theorem a_inv_pos_complete : forall a outT inT,
+    a_inv_pos a outT = inT ->
+    forall inT',
+      ArrowInvPos a outT inT' ->
+      inT <: inT'.
+Proof.
+  intros [T1 T2] outT inT Hinveq inT' Hinv.
+  unfold a_inv_pos in *. simpl in *.
+  destruct (IsEmpty_dec (tyAnd T2 outT)); subst; crush.
+  assert (exists v, IsA v (tyAnd T2 outT)) as Hex.
+  {
+    match goal with
+    | [H : IsInhabited _ |- _] => inversion i
+    end.
+    match goal with
+    | [H : IsA ?x (tyAnd T2 outT) |- _] => exists x; crush
+    end.
+  }
+  destruct Hex as [v Hv].
+  remember (fun (_:V) => Res v) as f.
+  (* f is a function that maps all T1 to 
+     som e value in (T2 ∩ outT) 
+   *)
+  assert (FnArrow f (Arrow inT T2)) as Hf.
+  {
+    constructor; intros.
+    right. exists v. crush.
+    inversion Hv. crush.
+  }
+  unfold Included. intros.
+  unfold ArrowInvPos in *.
+  apply (Hinv f Hf x v); crush.
+  inversion Hv; crush.
+Qed.
+
+Theorem a_inv_neg_complete : forall a outT inT,
+    a_inv_neg a outT = inT ->
+    forall inT',
+      ArrowInvNeg a outT inT'  ->
+      inT' <: inT.
+Proof.
+  intros [T1 T2] outT inT Hinv inT' H' x Hx.
+  unfold a_inv_neg in Hinv. simpl in *.
+  unfold ArrowInvNeg in *.
+  (* BOOKMARK STUCK *)
+
+  destruct (IsEmpty_dec (tyAnd T2 outT)) as [Hmt | Hnmt]; subst.
+  {
+    destruct (IsEmpty_dec outT) as [Homt | Honmt]; subst.
+    
+  }
+  
+  destruct (IsA_dec x inT); auto.
+  assert False.
+  {
+    
+  }
+  {
+    eapply H'.
+    (* we need a v in inT' s.t. (x)
+       f v = Res v' and
+       v' in outT  *)
+    unfold a_inv_neg in Hinv.
+    simpl in *.
+    destruct (IsEmpty_dec (tyAnd T2 outT)); subst.
+    simpl in *.
+  } 
+  ; crush.  
+  {
+    destruct (IsEmpty_dec outT).
+    {
+      (* if outT is empty...  *)
+    }
+    (* we need an f s.t. 
+       f : inT -> T2 *)
+    destruct (IsA_dec x inT); auto.
+    remember (fun (_:V) => Res x) as f.
+    
+
+    (* BOOKMARK *)
+    destruct (IsEmpty_dec T2); crush.
+    remember (fun (_:V) => Res x) as f.
+    assert (FnArrow f (Arrow inT T2)) as Hf.
+    {
+      constructor. intros v Hv.
+      crush.
+    }
+  }
+  {
+
+  }
+  
 Inductive interface : Type :=
 | IBase : arrow -> interface
 | ICons : arrow -> interface -> interface.
-
 Hint Constructors interface.
 
 Fixpoint i_dom (i : interface) : Ty :=
@@ -93,6 +282,7 @@ Fixpoint i_dom (i : interface) : Ty :=
   | IBase a => a_dom a
   | ICons a i' => tyOr (a_dom a) (i_dom i')
   end.
+Hint Unfold i_dom.
 
 Inductive FnInterface : fn -> interface -> Prop :=
 | FnIBase : forall f a,
@@ -136,17 +326,6 @@ Proof.
   induction Hi; crush.
 Qed.
 
-Ltac destruct_arrows :=
-  match goal with
-  | [a : arrow |- _] => destruct a
-  end.
-
-Ltac destruct_IsA :=
-  match goal with
-  | [H : IsA _ _ |- _] => destruct H
-  end.
-
-
 Lemma a_meet_arrow_fn : forall a a' f,
     FnArrow f a  ->
     FnArrow f a' ->
@@ -163,9 +342,7 @@ Proof with crush.
   match goal with
   | [H : _ _ = Res ?v |- _] => exists v; rewrite H in *
   end...
-  constructor; auto.
 Qed.
-
 Hint Resolve a_meet_arrow_fn.
 
   
@@ -193,163 +370,23 @@ Proof with crush.
 Qed.
 
 
-
-Definition overlap (t1 t2:Ty) : bool :=
-  if (IsEmpty_dec (tyAnd t1 t2)) then false else true.
-
-Hint Unfold overlap.
-
-Definition a_inv (a:arrow) (out:Ty) : Ty :=
-  if overlap (a_rng a) out
-  then (a_dom a)
-  else emptyTy.
-
-Hint Unfold a_inv.
-
-Definition ArrowInv
-           (a:arrow)
-           (outT inT : Ty) : Prop :=
-forall (f:fn),
-  FnArrow f a ->
-  forall (v v':V),
-    IsA v (a_dom a) ->
-    f v = Res v' ->
-    IsA v' outT ->
-    IsA v inT.
-
-Hint Unfold ArrowInv.
-
-Lemma no_overlap_empty : forall t1 t2,
-    false = overlap t1 t2 ->
-    IsEmpty (tyAnd t1 t2).
-Proof.
-  intros.
-  unfold overlap in *.
-  destruct (IsEmpty_dec (tyAnd t1 t2)); crush.
-Qed.
-
-Ltac same_Res :=
-  match goal with
-  | [H1 : ?f ?v = Res ?x , H2 : ?f ?v = Res ?y |- _] =>
-    rewrite H1 in H2; inversion H2; subst; clear H2
-  end.
-
-Ltac inv_FnArrow :=
-  match goal with
-  | [H : FnArrow _ _ |- _] => inversion H; subst
-  end.
-
-
-(* Arrow Inversion Soundness *)
-Theorem a_inv_sound : forall a outT inT,
-    a_inv a outT = inT ->
-    ArrowInv a outT inT.
-Proof with crush.
-  unfold ArrowInv.
-  intros.
-  destruct a as [T1 T2].
-  simpl in *.
-  unfold a_inv in *.
-  remember (overlap (a_rng (Arrow T1 T2)) outT) as Hoverlap.
-  ifcaseH...
-  inv_FnArrow.
-  applyHinH...
-  same_Res.
-  forwards: no_overlap_empty. eauto.
-  unfold IsEmpty in *.
-  assert (Inhabited V (tyAnd T2 outT)).
-  apply (Inhabited_intro _ _ x). unfold tyAnd... crush.
-Qed.
-
-Lemma no_empty_val : forall v,
-    ~ IsA v emptyTy.
-Proof.
-  intros v Hmt. inversion Hmt.
-Qed.
-  
-Lemma empty_no_overlap_l : forall T T',
-    IsEmpty T -> overlap T T' = false.
-Proof.
-  intros T T' Hmt.
-  unfold overlap.
-  ifcase. auto.
-  assert False.
-  intuition.
-  applyH.
-  unfold IsEmpty in *.
-  intros Hin.
-  inversion Hin as [v Hv].
-  inversion Hv; subst.
-  apply Hmt. apply (Inhabited_intro V T v).
-  auto.
-  crush.
-Qed.
-  
-Lemma not_empty_exists : forall T,
-    ~ IsEmpty T ->
-    exists v, IsA v T.
-Proof.
-  intros T HTmt.
-  unfold IsEmpty in *.
-  apply NNPP in HTmt.
-  inversion HTmt.
-  eexists. eauto.
-Qed.
-  
-  
-(* Arrow Inversion Completeness *)
-Theorem a_inv_complete : forall a outT inT,
-    a_inv a outT = inT ->
-    forall inT',
-      ArrowInv a outT inT' ->
-      inT <: inT'.
-Proof.
-  intros a outT intT Hinveq inT' Hinv.
-  destruct a as [T1 T2].
-  unfold a_inv in *. simpl in *.
-  unfold overlap in *.
-  remember (IsEmpty_dec (tyAnd T2 outT)) as Hmt.
-  destruct Hmt as [Hmt | Hnmt].
-  (* IsEmpty (tyAnd T2 outT) *)
-  {
-    subst. unfold Included; intros.
-    assert False. eapply no_empty_val. eassumption. crush.
-  }
-  (* ~ IsEmpty (tyAnd T2 outT) *)
-  {
-    assert (exists v, IsA v (tyAnd T2 outT)) as Hex.
-    apply not_empty_exists. auto. destruct Hex as [v Hv].
-    remember (fun (_:V) => Res v) as f.
-    (* f is a function that maps all T1 to 
-       some value in (T2 ∩ outT) 
-      *)
-    assert (FnArrow f (Arrow T1 T2)) as Hf.
-    {
-     constructor; intros.
-     right. exists v. crush.
-     inversion Hv. crush.
-    }
-    unfold Included. intros.
-    unfold ArrowInv in *.
-    apply (Hinv f Hf x v); crush.
-    inversion Hv; crush.
-  }
-Qed.
-
-
-
-Fixpoint i_inv_aux (p: interface) (out:Ty) : Ty :=
+Fixpoint i_inv_pos (p: interface) (out:Ty) : Ty :=
   match p with
-  | IBase a => (a_inv a out)
-  | ICons a p' => tyOr (a_inv a out) (i_inv_aux p' out)
+  | IBase a => (a_inv_pos a out)
+  | ICons a p' => tyOr (a_inv_pos a out) (i_inv_pos p' out)
   end.
 
+Fixpoint i_inv_neg (p: interface) (out:Ty) : Ty :=
+  match p with
+  | IBase a => (a_inv_neg a out)
+  | ICons a p' => tyOr (a_inv_neg a out) (i_inv_neg p' out)
+  end.
 Definition i_inv (i:interface) (out:Ty) : Ty :=
   let p := (i_powerset i) in
-  let pos := i_inv_aux p out in
-  let neg := i_inv_aux p (tyNot out) in
+  let pos := i_inv_pos p out in
+  let neg := i_inv_neg p (tyNot out) in
   tyDiff pos neg.
-
+Hint Unfold i_inv i_inv_aux i_app i_map i_powerset.
 
 
 Definition InterfaceInv
@@ -363,17 +400,97 @@ forall (f:fn),
     IsA v' outT ->
     IsA v inT.
 
+Ltac inv_FnInterface :=
+  match goal with
+  | [H : FnInterface _ _ |- _] => inversion H; subst
+  end.
+
+Lemma in_tyDiff : forall v T1 T2,
+    IsA v T1 ->
+    ~ IsA v T2 ->
+    IsA v (tyDiff T1 T2).
+Proof.
+  crush.
+Qed.
+
 
 (* Interface Inversion Soundness *)
-Theorem i_inv_sound : forall i outT inT,
+Lemma i_inv_sound : forall i outT inT,
       i_inv i outT = inT ->
-      InterfaceInv i inT outT.
-Proof.
+      InterfaceInv i outT inT.
+Proof with crush.
+  intros i; induction i.
+  (* i =  (IBase a) *)
+  {
+    intros outT inT Hinv f Hint v v' Hv Hf Hv'.
+    destruct a as [T1 T2].
+    inv_FnInterface...
+    inv_FnArrow.
+    assert (IsA v T1) as temp; auto.
+    applyIn temp...
+    same_Res.
+    unfold i_inv. unfold i_powerset. unfold i_inv_aux.
+    apply in_tyDiff.
+    (* Goal:  IsA v (a_inv (Arrow T1 T2) outT) *)
+    {
+      eapply a_inv_sound; eauto.
+    }
+    (* Goal: ~ IsA v (a_inv (Arrow T1 T2) (tyNot outT)) *)
+    {
+      unfold a_inv in *. simpl in *.
+      intro Hv''.
+      destruct (IsEmpty_dec (tyAnd T2 (tyNot outT))).
+      {
+        eapply no_empty_val. eassumption.
+      }
+      {
+        assert ().
+        match goal with
+        | [H : IsInhabited _ |- _] => inversion H
+        end.
+        inv_FnArrow.
+        assert (f v = Bot \/ (exists v' : V, IsA v' T2 /\ f v = Res v'))
+          as Habsurd. auto.
+        inversion Habsurd; subst. crush.
+        match goal with
+        | [H : IsInhabited _ |- _] => inversion H
+        end.
+        
+      }
+      eapply a_inv_sound in H1; eauto.
+      eapply H1 in Hv'.
+    }
+    
+    unfold Setminus.
+    unfold a_inv. simpl in *.
+    ifcase. crush.
+    ifcase.
+    cbv.
+    intros.
+    
+    crush.
+    
+     (@a_inv_sound (Arrow T1 T2) outT).
+    simpl in *.
+  }
+  (* i =  (ICons a i') *)
+  {
+  }
+  intros i outT inT Hinv f Hint v v' Hv Hf Hv'...
+  inv_FnInterface...
+  (* FnInterface f (IBase a) *)
+  {
+    
+  }
+  (* FnInterface f (ICons a) *)
+  {
+
+  }
   Admitted.
   
 
 (* Interface Inversion Completeness *)
-Theorem i_inv_complete : forall i outT inT,
+Lemma i_inv_complete : forall i outT inT,
     i_inv i outT = inT ->
     forall inT',
       InterfaceInv i outT inT' ->
